parameterize hist by event

newio/Hist.fst
@@ -1,27 +1,24 @@
 module Hist
 
-
 open FStar.Tactics
 open FStar.List.Tot.Base
 
 (** The postcondition for an io computation is defined over the
-result (type: a) and local trace (type: trace).
+result (type: a) and local trace (type: list event).
 The local trace represents the events that happend during the
 computation. Local trace is in chronological order.
 
-We also have the history (type: trace) that represents the
+We also have the history (type: list event) that represents the
 events that happend until the beginning of the io computation.
 The history is in reverse chronological order.
 
 At the end of an io computation, the local trace is
 reversed and appended to the history. **)
 
-let trace = Free.IO.trace
+let hist_post (#event) a = lt:list event -> r:a -> Type0
+let hist_pre (#event) = h:list event -> Type0
 
-let hist_post a = lt:trace -> r:a -> Type0
-let hist_pre = h:trace -> Type0
-
-private let hist0 a = hist_post a -> hist_pre
+private let hist0 (#event) a = hist_post #event a -> hist_pre #event
 
 unfold
 let hist_post_ord (p1 p2:hist_post 'a) = forall lt r. p1 lt r ==> p2 lt r
@@ -29,26 +26,23 @@ let hist_post_ord (p1 p2:hist_post 'a) = forall lt r. p1 lt r ==> p2 lt r
 let hist_wp_monotonic (wp:hist0 'a) =
   forall p1 p2. (p1 `hist_post_ord` p2) ==> (forall h. wp p1 h ==> wp p2 h)
 
-let hist a = wp:(hist0 a){hist_wp_monotonic wp}
+let hist #event a = wp:(hist0 #event a){hist_wp_monotonic wp}
 
 let hist_return (x:'a) : hist 'a =
   fun p _ -> p [] x
 
 unfold
-let hist_post_shift (p:hist_post 'a) (lt:trace) : hist_post 'a =
+let hist_post_shift (p:hist_post 'a) (lt:list 'event) : hist_post 'a =
   fun lt' r -> p (lt @ lt') r
 
 unfold
-let trace_append (h lt:trace) = List.rev lt @ h
-
-unfold
 let hist_post_bind
-  (h:trace)
+  (h:list 'event)
   (kw : 'a -> hist 'b)
   (p:hist_post 'b) :
   Tot (hist_post 'a) =
   fun lt r ->
-    kw r (hist_post_shift p lt) (trace_append h lt)
+    kw r (hist_post_shift p lt) (List.rev lt @ h)
 
 unfold
 let hist_bind (w : hist 'a) (kw : 'a -> hist 'b) : hist 'b =
@@ -60,7 +54,7 @@ let wp_lift_pure_hist (w : pure_wp 'a) : hist 'a =
   fun p _ -> w (p [])
 
 unfold
-val hist_ord (#a : Type) : hist a -> hist a -> Type0
+val hist_ord (#event:Type) (#a : Type) : hist #event a -> hist #event a -> Type0
 let hist_ord wp1 wp2 = forall h p. wp1 p h ==> wp2 p h
 
 unfold
